ContextAlgebra/theories/ResourceExtensionEquiv.v
@@ -1,6 +1,6 @@
 (** * Fiber extension equivalence and commuting lemmas *)
 
-From ContextBase Require Import Prelude LogicVarInterface.
+From ContextBase Require Import Prelude LogicVar.
 From ContextStore Require Import Store.
 From ContextAlgebra Require Import ResourceCore ResourceKeyAction ResourceRestrict
   ResourceAlgebra ResourceExtensionCore.
