ContextStore/StoreInterfaceRestrict.v
@@ -1,6 +1,6 @@
 (** * Concrete store restriction interface lemmas *)
 
-From ContextBase Require Import Prelude LogicVarInterface.
+From ContextBase Require Import Prelude LogicVar.
 From ContextStore Require Import StoreCore StoreKeyAction StoreRestrictCore StoreRestrictUnion StoreBind.
 From ContextStore Require Export StoreInterfaceLookupSwap.
 
